\documentclass[12pt,answers]{exam}
\usepackage{ctex}
\usepackage{amsmath}
\begin{document}
\section*{关于求和}
\begin{questions}
\question 求 $1+2+\cdots n$ 
\question 求 $1^2+2^2+\cdots+n^2$
\question 求和$\sum_{i}^{k} f(i)$,表示 $f(i)+f(i+1)+\cdots +f(k)$,因此问题
\begin{parts}
\part 1可以写成$\sum_{i}^{n} i$
\part 2 可以写成 $\sum_{i}^{n}i^2$
\end{parts}
\begin{solution}
\[\sum_{i=1}^{n} i=\frac{n(n+1)}{2}\]
\end{solution}
\begin{solution}
\[\sum_{i=1}^{n} i^2=\frac{n(n+1)(2n+1)}{6}\]
提供一种计算方法,由
\[ (i+1)^3-i^3 =i^3+3i+3i^2+1-i^3=3i+3i^2+1\]
得
\[\sum_{i=1}^{n} \{(i+1)^3-i^3\}=\sum_{i=1}^{n}\{3i+3i^2+1\}\]
而 \[\sum_{i=1}^{n}\{(i+1)^3-i^3\} =\sum_{i=2}^{n+1}i^3 -\sum_{i=1}^{n}i^3=(n+1)^3-1 \]
\[\sum_{i=1}^{n} \{3i+3i^2+1\} =\sum_{i=1}^{n}3i^2+\frac{n(3n+5)}{2}\]
所以 \[\sum_{i=1}^{n}i^2 = \frac{(n+1)^3-1}{3} -\frac{n(3n+5)}{6}=\frac{n(n+1)(2n+1)}{6}\]
\end{solution}
\end{questions}

\end{document}